try with copy of U64

Clean/Gadgets/Rotation64/Rotation64.lean
@@ -25,12 +25,8 @@ def rot64 (offset : Fin 64) (x : Var U64 (F p)) : Circuit (F p) (Var U64 (F p)) 
   let byte_offset := offset / 8
   let bit_offset : ℕ := (offset % 8).val
 
-  -- apply the byte rotation
-  let out ← subcircuit (Gadgets.Rotation64Bytes.circuit byte_offset) x
-
   -- apply the bit rotation
-
-  let ⟨low, high⟩ ← subcircuit (Gadgets.U64ByteDecomposition.circuit bit_offset) out
+  let ⟨low, high⟩ ← subcircuit (Gadgets.U64ByteDecomposition.circuit bit_offset) x
   let ⟨x0_l, x1_l, x2_l, x3_l, x4_l, x5_l, x6_l, x7_l⟩ := low
   let ⟨x0_h, x1_h, x2_h, x3_h, x4_h, x5_h, x6_h, x7_h⟩ := high
 
@@ -44,7 +40,11 @@ def rot64 (offset : Fin 64) (x : Var U64 (F p)) : Circuit (F p) (Var U64 (F p)) 
   assert_zero (x6_l * ((2 : ℕ)^(8 - bit_offset) : F p) + x5_h - y5)
   assert_zero (x7_l * ((2 : ℕ)^(8 - bit_offset) : F p) + x6_h - y6)
   assert_zero (x0_l * ((2 : ℕ)^(8 - bit_offset) : F p) + x7_h - y7)
-  return ⟨ y0, y1, y2, y3, y4, y5, y6, y7 ⟩
+
+  -- apply the byte rotation
+  let y ← subcircuit (Gadgets.Rotation64Bytes.circuit byte_offset) ⟨y0, y1, y2, y3, y4, y5, y6, y7⟩
+  let out ← U64.copy y
+  return out
 
 instance lawful (off : Fin 64) : ConstantLawfulCircuits (F := (F p)) (rot64 off) := by infer_constant_lawful_circuits
 
@@ -54,10 +54,12 @@ def spec (offset : Fin 64) (x : U64 (F p)) (y: U64 (F p)) :=
   y.value = rot_right64 x.value offset.val
   ∧ y.is_normalized
 
+#eval! (rot64 (p:=p_babybear) 0) default |>.operations.local_length
+#eval! (rot64 (p:=p_babybear) 0) default |>.output
 def elaborated (off : Fin 64) : ElaboratedCircuit (F p) U64 (Var U64 (F p)) where
   main := rot64 off
-  local_length _ := 24
-  output _inputs i0 := var_from_offset U64 (i0 + 16)
+  local_length _ := 32
+  output _inputs i0 := var_from_offset U64 (i0 + 24)
   initial_offset_eq := by
     intros
     simp only [rot64]
@@ -71,10 +73,9 @@ def elaborated (off : Fin 64) : ElaboratedCircuit (F p) U64 (Var U64 (F p)) wher
 theorem soundness (offset : Fin 64) : Soundness (F p) (circuit := elaborated offset) assumptions (spec offset) := by
   intro i0 env ⟨x0_var, x1_var, x2_var, x3_var, x4_var, x5_var, x6_var, x7_var ⟩ ⟨x0, x1, x2, x3, x4, x5, x6, x7⟩ h_input x_byte h_holds
 
-  simp [elaborated, subcircuit_norm, rot64, Circuit.constraints_hold.soundness] at h_holds
-
-  rw [Circuit.constraints_hold.bind_soundness (by infer_lawful_circuit) (by infer_lawful_circuit)] at h_holds
-
+  simp [elaborated, subcircuit_norm, rot64, Circuit.constraints_hold.soundness, U64.witness] at h_holds
+  -- simp [circuit_norm, subcircuit_norm, U64ByteDecomposition.circuit, U64ByteDecomposition.elaborated,
+  -- Rotation64Bytes.circuit, Rotation64Bytes.elaborated] at h_holds
   sorry
 
 theorem completeness (offset : Fin 64) : Completeness (F p) (circuit := elaborated offset) U64 assumptions := by
